execution/theories/Extras.v
@@ -1016,10 +1016,10 @@ Proof.
   destruct (g (f x)); auto.
 Qed.
 
-Lemma map_eq_2 {A B C} (f : A -> C) (g : B -> C) (xs : list A) (ys : list B) :
+Lemma list_eq_nth {A} (xs ys : list A) :
   length xs = length ys ->
-  (forall i a b, nth_error xs i = Some a -> nth_error ys i = Some b -> f a = g b) ->
-  map f xs = map g ys.
+  (forall i a a', nth_error xs i = Some a -> nth_error ys i = Some a' -> a = a') ->
+  xs = ys.
 Proof.
   revert ys.
   induction xs as [|x xs IH]; intros ys len_xs all_eq.
@@ -1032,6 +1032,19 @@ Proof.
     + lia.
     + intros i a b ntha nthb.
       apply all_eq with (S i); cbn; auto.
+Qed.
+
+Lemma nth_error_seq_in i start len :
+  i < len ->
+  nth_error (seq start len) i = Some (start + i).
+Proof.
+  revert i start.
+  induction len as [|len IH]; intros i start ilt; try lia.
+  cbn.
+  destruct i as [|i]; cbn.
+  - f_equal; lia.
+  - rewrite IH by lia.
+    f_equal; lia.
 Qed.
 
 (*
@@ -1053,6 +1066,16 @@ Proof.
     rewrite perm in H.
     apply in_iff.
 *)
+
+Lemma f_match_option {A B C} (f : A -> B) (o : option C) a b :
+  f match o with
+    | Some x => a
+    | None => b
+    end = match o with
+          | Some x => f a
+          | None => f b
+          end.
+Proof. destruct o; auto. Qed.
 
 Definition large_modulus : Z :=
 32317006071311007300338913926423828248817941241140239112842009751400741706634354222619689417363569347117901737909704191754605873209195028853758986185622153212175412514901774520270235796078236248884246189477587641105928646099411723245426622522193230540919037680524235519125679715870117001058055877651038861847280257976054903569732561526167081339361799541336476559160368317896729073178384589680639671900977202194168647225871031411336429319536193471636533209717077448227988588565369208645296636077250268955505928362751121174096972998068410554359584866583291642136218231078990999448652468262416972035911852507045361090559.
